Foundation/Modal/Neighborhood/AxiomC.lean
@@ -1,0 +1,30 @@
+import Foundation.Modal.Tableau
+import Foundation.Modal.Neighborhood.Basic
+
+namespace LO.Modal.Neighborhood
+
+open Formula.Neighborhood
+
+variable {F : Frame}
+
+class Frame.IsRegular (F : Frame) : Prop where
+  regular : ∀ X Y : Set F, (F.η X) ∩ (F.η Y) ⊆ F.η (X ∩ Y)
+
+lemma Frame.regular [Frame.IsRegular F] {X Y : Set F} : (F.η X) ∩ (F.η Y) ⊆ F.η (X ∩ Y) := by apply IsRegular.regular
+
+instance : Frame.trivial.IsRegular := ⟨by tauto_set⟩
+
+lemma valid_axiomC_of_isRegular [F.IsRegular] : F ⊧ Axioms.C (.atom 0) (.atom 1) := by
+  intro V x;
+  simp only [
+    Satisfies, Model.truthset.eq_imp, Model.truthset.eq_and, Model.truthset.eq_box,
+    Model.truthset.eq_atom, Set.mem_union, Set.mem_compl_iff, Set.mem_inter_iff, Set.mem_setOf_eq
+  ];
+  apply not_or_of_imp;
+  rintro ⟨h₁, h₂⟩;
+  apply F.regular;
+  constructor;
+  . apply h₁;
+  . apply h₂;
+
+end LO.Modal.Neighborhood
