Foundation/Modal/Neighborhood/AxiomM.lean
@@ -1,0 +1,28 @@
+import Foundation.Modal.Tableau
+import Foundation.Modal.Neighborhood.Basic
+
+namespace LO.Modal.Neighborhood
+
+open Formula.Neighborhood
+
+variable {F : Frame}
+
+class Frame.IsMonotonic (F : Frame) : Prop where
+  mono : ∀ X Y : Set F, X ⊆ Y → F.η X ⊆ F.η Y
+
+lemma Frame.mono [Frame.IsMonotonic F] {X Y : Set F} : X ⊆ Y → F.η X ⊆ F.η Y := by apply IsMonotonic.mono
+
+instance : Frame.trivial.IsMonotonic := ⟨by simp⟩
+
+lemma valid_axiomM_of_isMonotonic [F.IsMonotonic] : F ⊧ Axioms.M (.atom 0) (.atom 1) := by
+  intro V x;
+  simp only [
+    Satisfies, Model.truthset.eq_imp, Model.truthset.eq_box, Model.truthset.eq_and,
+    Model.truthset.eq_atom, Set.mem_union, Set.mem_compl_iff, Set.mem_setOf_eq, Set.mem_inter_iff
+  ]
+  apply not_or_of_imp;
+  intro h;
+  constructor <;>
+  . apply F.mono (by simp) h;
+
+end LO.Modal.Neighborhood
