Foundation/Modal/Neighborhood/Logic/E.lean
@@ -21,62 +21,6 @@ instance : Entailment.Consistent Hilbert.E := consistent_of_sound_frameclass Fra
   use ⟨Unit, λ _ => {}⟩;
   simp;
 
-instance : Hilbert.E ⪱ Hilbert.EC := by
-  constructor;
-  . apply Hilbert.WithRE.weakerThan_of_subset_axioms;
-    simp;
-  . apply Entailment.not_weakerThan_iff.mpr;
-    use (Axioms.C (.atom 0) (.atom 1));
-    constructor;
-    . simp;
-    . apply Sound.not_provable_of_countermodel (𝓜 := FrameClass.E);
-      apply not_validOnFrameClass_of_exists_model_world;
-      let M : Model := {
-        World := Fin 2,
-        ν := λ w =>
-          match w with
-          | 0 => {{0}, {1}}
-          | 1 => {∅},
-        Val := λ w =>
-          match w with
-          | 0 => {0}
-          | 1 => {1}
-          | _ => Set.univ
-      };
-      use M, 0;
-      constructor;
-      . tauto;
-      . simp [M, Semantics.Realize, Satisfies]
-
-instance : Hilbert.E ⪱ Hilbert.EM := by
-  constructor;
-  . apply Hilbert.WithRE.weakerThan_of_subset_axioms;
-    simp;
-  . apply Entailment.not_weakerThan_iff.mpr;
-    use (Axioms.M (.atom 0) (.atom 1));
-    constructor;
-    . simp;
-    . apply Sound.not_provable_of_countermodel (𝓜 := FrameClass.E);
-      apply not_validOnFrameClass_of_exists_model_world;
-      let M : Model := {
-        World := Fin 3,
-        ν := λ w =>
-          match w with
-          | 0 => {{1}, {2}, {0, 2}}
-          | 1 => {{0, 1}, {0, 2}, {0}}
-          | 2 => {{0}, {1, 2}, ∅},
-        Val := λ w =>
-          match w with
-          | 0 => {0, 1}
-          | 1 => {1, 2}
-          | _ => Set.univ
-      };
-      use M, 0;
-      constructor;
-      . tauto;
-      . simp! [M, Semantics.Realize, Satisfies];
-        tauto_set;
-
 instance : Hilbert.E ⪱ Hilbert.EK := by
   constructor;
   . apply Hilbert.WithRE.weakerThan_of_subset_axioms;
@@ -133,8 +77,6 @@ instance : Hilbert.E ⪱ Hilbert.EN := by
 
 end Hilbert.E.Neighborhood
 
-instance : 𝐄 ⪱ 𝐄𝐌 := inferInstance
-instance : 𝐄 ⪱ 𝐄𝐂 := inferInstance
 instance : 𝐄 ⪱ 𝐄𝐍 := inferInstance
 instance : 𝐄 ⪱ 𝐄𝐊 := inferInstance
 
