Foundation/Modal/Neighborhood/Logic/EC.lean
@@ -1,0 +1,67 @@
+import Foundation.Modal.Neighborhood.Hilbert
+import Foundation.Modal.Neighborhood.AxiomC
+import Foundation.Modal.Neighborhood.Logic.E
+
+namespace LO.Modal
+
+open Neighborhood
+open Hilbert.Neighborhood
+open Formula.Neighborhood
+
+namespace Neighborhood
+
+@[reducible] protected alias Frame.IsEC := Frame.IsRegular
+protected abbrev FrameClass.EC : FrameClass := { F | F.IsEC }
+
+end Neighborhood
+
+
+namespace Hilbert
+
+namespace EC.Neighborhood
+
+instance : Sound Hilbert.EC FrameClass.EC := instSound_of_validates_axioms $ by
+  simp only [Semantics.RealizeSet.singleton_iff];
+  intro F hF;
+  replace hF := Set.mem_setOf_eq.mp hF;
+  apply valid_axiomC_of_isRegular;
+
+instance : Entailment.Consistent Hilbert.EC := consistent_of_sound_frameclass FrameClass.EC $ by
+  use Frame.trivial;
+  simp only [Set.mem_setOf_eq];
+  infer_instance;
+
+end EC.Neighborhood
+
+instance : Hilbert.E ⪱ Hilbert.EC := by
+  constructor;
+  . apply Hilbert.WithRE.weakerThan_of_subset_axioms;
+    simp;
+  . apply Entailment.not_weakerThan_iff.mpr;
+    use (Axioms.C (.atom 0) (.atom 1));
+    constructor;
+    . simp;
+    . apply Sound.not_provable_of_countermodel (𝓜 := FrameClass.E);
+      apply not_validOnFrameClass_of_exists_model_world;
+      let M : Model := {
+        World := Fin 2,
+        ν := λ w =>
+          match w with
+          | 0 => {{0}, {1}}
+          | 1 => {∅},
+        Val := λ w =>
+          match w with
+          | 0 => {0}
+          | 1 => {1}
+          | _ => Set.univ
+      };
+      use M, 0;
+      constructor;
+      . tauto;
+      . simp [M, Semantics.Realize, Satisfies]
+
+end Hilbert
+
+instance : 𝐄 ⪱ 𝐄𝐂 := inferInstance
+
+end LO.Modal
