Foundation/Modal/Neighborhood/Logic/EMC.lean
@@ -1,0 +1,150 @@
+import Foundation.Modal.Neighborhood.Hilbert
+import Foundation.Modal.Neighborhood.Logic.EM
+import Foundation.Modal.Neighborhood.Logic.EC
+
+
+lemma _root_.Set.powerset_Fin2 : Set.powerset (Set.univ : Set (Fin 2)) = {{0, 1}, {0}, {1}, ∅} := by
+  ext x;
+  simp only [Set.powerset_univ, Set.mem_univ, Fin.isValue, Set.mem_insert_iff, Set.mem_singleton_iff, true_iff];
+  by_cases h0 : 0 ∈ x <;>
+  by_cases h1 : 1 ∈ x;
+  . left;
+    ext i;
+    match i with | 0 | 1 => simp_all;
+  . right; left;
+    ext i;
+    match i with | 0 | 1 => simp_all;
+  . right; right; left;
+    ext i;
+    match i with | 0 | 1 => simp_all;
+  . right; right; right;
+    ext i;
+    match i with | 0 | 1 => simp_all;
+
+lemma _root_.Set.all_cases_Fin2 (s : Set (Fin 2)) : s = {0, 1} ∨ s = {0} ∨ s = {1} ∨ s = ∅ := by
+  simpa using Set.powerset_Fin2.subset (by simp);
+
+
+namespace LO.Modal
+
+open Neighborhood
+open Hilbert.Neighborhood
+open Formula.Neighborhood
+
+namespace Neighborhood
+
+protected class Frame.IsEMC (F) extends Frame.IsMonotonic F, Frame.IsRegular F where
+protected abbrev FrameClass.EMC : FrameClass := { F | F.IsEMC }
+
+end Neighborhood
+
+
+namespace Hilbert
+
+namespace EMC.Neighborhood
+
+instance : Sound Hilbert.EMC FrameClass.EMC := instSound_of_validates_axioms $ by
+  simp only [Semantics.RealizeSet.insert_iff, Semantics.RealizeSet.singleton_iff];
+  refine ⟨?_, ?_⟩;
+  . intro F hF;
+    replace hF := Set.mem_setOf_eq.mp hF;
+    apply valid_axiomM_of_isMonotonic;
+  . intro F hF;
+    replace hF := Set.mem_setOf_eq.mp hF;
+    apply valid_axiomC_of_isRegular;
+
+instance : Entailment.Consistent Hilbert.EMC := consistent_of_sound_frameclass FrameClass.EMC $ by
+  use Frame.trivial;
+  simp;
+  constructor;
+
+end EMC.Neighborhood
+
+instance : Hilbert.EC ⪱ Hilbert.EMC := by
+  constructor;
+  . apply Hilbert.WithRE.weakerThan_of_subset_axioms;
+    simp;
+  . apply Entailment.not_weakerThan_iff.mpr;
+    use (Axioms.M (.atom 0) (.atom 1));
+    constructor;
+    . simp;
+    . apply Sound.not_provable_of_countermodel (𝓜 := FrameClass.EC);
+      apply not_validOnFrameClass_of_exists_model_world;
+      let M : Model := {
+        World := Fin 3,
+        ν := λ w =>
+          match w with
+          | 0 => {{1}}
+          | 1 => {{0}, {0, 1}}
+          | 2 => {{0}, {1, 2}, ∅},
+        Val := λ w =>
+          match w with
+          | 0 => {0, 1}
+          | 1 => {1, 2}
+          | _ => Set.univ
+      };
+      use M, 0;
+      constructor;
+      . exact {
+          regular := by
+            rintro X Y w ⟨hwX, hwY⟩;
+            match w with
+            | 0 => simp_all [M];
+            | 1 =>
+              rcases hwX with (rfl | rfl) <;>
+              rcases hwY with (rfl | rfl) <;>
+              simp_all [M];
+            | 2 =>
+              rcases hwX with (rfl | rfl | rfl) <;>
+              rcases hwY with (rfl | rfl | rfl) <;>
+              simp [M]
+        }
+      . simp! [M, Semantics.Realize, Satisfies];
+        ext x;
+        simp;
+        omega;
+
+instance : Hilbert.EM ⪱ Hilbert.EMC := by
+  constructor;
+  . apply Hilbert.WithRE.weakerThan_of_subset_axioms;
+    simp;
+  . apply Entailment.not_weakerThan_iff.mpr;
+    use (Axioms.C (.atom 0) (.atom 1));
+    constructor;
+    . simp;
+    . apply Sound.not_provable_of_countermodel (𝓜 := FrameClass.EM);
+      apply not_validOnFrameClass_of_exists_model_world;
+      let M : Model := {
+        World := Fin 2,
+        ν := λ w =>
+          match w with
+          | 0 => {{0}, {1}, {0, 1}}
+          | 1 => {{1}, {0, 1}},
+        Val := λ w =>
+          match w with
+          | 0 => {0}
+          | 1 => {1}
+          | _ => Set.univ
+      };
+      use M, 0;
+      constructor;
+      . exact {
+          mono := by
+            rintro X Y hXY w hwX;
+            match w with
+            | 0 | 1 =>
+              rcases hwX with rfl | rfl | rfl <;>
+              rcases Set.all_cases_Fin2 Y with rfl | rfl | rfl | rfl <;>
+              tauto_set;
+        }
+      . simp! [M, Semantics.Realize, Satisfies];
+        by_contra! h;
+        have := h.symm.subset';
+        simp at this;
+
+end Hilbert
+
+instance : 𝐄𝐂 ⪱ 𝐄𝐌𝐂 := inferInstance
+instance : 𝐄𝐌 ⪱ 𝐄𝐌𝐂 := inferInstance
+
+end LO.Modal
